src/Primitive/Prim/Ber_decode_primitive.v
@@ -39,28 +39,47 @@ Definition prim_enc_res td  sl buf_size li :=
 Definition prim_type_s := (Tstruct _ASN__PRIMITIVE_TYPE_s noattr).
 Definition mk_prim_type_s (buf_p : val) struct_len := (buf_p, Vint (Int.repr struct_len)).
 
+Definition Z_of_val v := 
+  match v with
+  | Vptr b i => Ptrofs.unsigned i 
+  | _ => 0
+  end.
+
 Definition ber_decode_primitive_spec : ident * funspec :=
   DECLARE _ber_decode_primitive
     WITH ctx_p : val, ctx : Z, td_p : val, td : TYPE_descriptor,
          st_pp : val, buf_p : val, buf : list Z,
-         res_p : val, size : Z, tag_mode : Z, st_p : val 
+         res_p : val, size : Z, tag_mode : Z, st_p : val, tags_p : val
     PRE [tptr asn_dec_rval_s, tptr asn_codec_ctx_s, tptr type_descriptor_s,
           tptr (tptr tvoid), tptr tvoid, tuint, tint] 
       PROP (is_pointer_or_null st_p;
             tag_mode = 0;
             0 <= size <= Int.max_signed;
             Zlength buf = size;
-            isptr buf_p)
+            isptr buf_p;
+           0 < Zlength buf <= Ptrofs.max_unsigned;
+           Z.land (Znth 0 buf) 32 = 0; 
+           1 = Zlength (tags td) ;
+           0 <= Z_of_val buf_p + Zlength buf <= Ptrofs.max_unsigned;
+           Forall (fun x : Z => 0 <= x <= Byte.max_unsigned) buf)
+
       PARAMS (res_p; ctx_p; td_p; st_pp; buf_p; Vint (Int.repr size);
                 Vint (Int.repr tag_mode))
       GLOBALS ()
       SEP (valid_pointer st_p;
-          if eq_dec st_p nullval 
+           if eq_dec st_p nullval 
            then emp
-           else data_at_ Ews tint st_p ; 
+           else data_at_ Ews (Tstruct _ASN__PRIMITIVE_TYPE_s noattr) st_p ; 
            (* need ctx value for ber_check_tags *)
            data_at Tsh asn_codec_ctx_s (Vint (Int.repr ctx)) ctx_p;
-           data_at_ Tsh type_descriptor_s td_p;
+           data_at Tsh (tarray tuint (Zlength (tags td)))
+                  (map Vint (map Int.repr (tags td))) tags_p;
+           field_at Tsh (Tstruct ber_decoder._asn_TYPE_descriptor_s noattr)
+                    (DOT ber_decoder._tags) tags_p td_p ;
+           field_at Tsh (Tstruct ber_decoder._asn_TYPE_descriptor_s noattr)
+                   (DOT ber_decoder._tags_count)
+                   (Vint (Int.repr (Zlength (tags td))))
+        td_p; 
            data_at Tsh (tarray tuchar (Zlength buf)) (map Vint (map Int.repr buf)) buf_p;
            data_at Tsh (tptr tvoid) st_p st_pp;
            data_at_ Tsh asn_dec_rval_s res_p)
@@ -71,25 +90,52 @@ Definition ber_decode_primitive_spec : ident * funspec :=
         (* Unchanged *)
          valid_pointer st_p;
          data_at Tsh asn_codec_ctx_s (Vint (Int.repr ctx)) ctx_p;
-         data_at_ Tsh type_descriptor_s td_p;
+         data_at Tsh (tarray tuint (Zlength (tags td)))
+                  (map Vint (map Int.repr (tags td))) tags_p;
+      field_at Tsh (Tstruct ber_decoder._asn_TYPE_descriptor_s noattr)
+                    (DOT ber_decoder._tags) tags_p td_p ;
+      field_at Tsh (Tstruct ber_decoder._asn_TYPE_descriptor_s noattr)
+                   (DOT ber_decoder._tags_count)
+                   (Vint (Int.repr (Zlength (tags td))))
+        td_p; 
          data_at Tsh (tarray tuchar (Zlength buf)) (map Vint (map Int.repr buf)) buf_p;
          (* Changed according to spec *)
-         let RC_FAIL := data_at Tsh asn_dec_rval_s (Vint (Int.repr 2), Vzero) res_p in
-         EX v : val, EX ls : list val,
+         let RC_FAIL := 
+             data_at Tsh asn_dec_rval_s (Vint (Int.repr 2), Vzero) res_p in
+         EX v : val, EX buf_p : val,
              data_at Tsh (tptr tvoid) v st_pp *
              if eq_dec v nullval 
              then RC_FAIL  
              else match primitive_decoder td ctx size (sizeof tuint)
-                                          Int.max_unsigned (map Byte.repr buf) with
+                        Int.modulus (map Byte.repr buf) with
                   | Some (r, c) => 
                     data_at Tsh asn_dec_rval_s (Vzero, Vint (Int.repr c)) res_p *
-                    data_at Ews (tarray tint (Zlength r)) (map Vubyte r) v
+                    data_at Tsh (tarray tuint (Zlength r)) (map Vubyte r) buf_p *
+                    data_at Ews (Tstruct _ASN__PRIMITIVE_TYPE_s noattr)
+                            (buf_p, Vint (Int.repr (Zlength r))) v
                   | None =>
                     RC_FAIL * 
-                    data_at Ews (tarray tint (Zlength ls)) ls v 
+                    data_at_ Ews (Tstruct _ASN__PRIMITIVE_TYPE_s noattr) v 
                   end).
 
-Definition Gprog := ltac:(with_library prog [(_calloc, calloc_spec);
+Definition calloc_spec_prim {cs : compspecs} :=
+   WITH m : Z, n : Z, t : type
+   PRE [ size_t, size_t ]
+       PROP (0 <= m <= Ptrofs.max_unsigned ;
+             0 <= n <= Ptrofs.max_unsigned ;
+             0 <= m * n <= Ptrofs.max_unsigned;
+             sizeof t = n)
+       PARAMS (Vptrofs (Ptrofs.repr m); 
+               Vptrofs (Ptrofs.repr n)) 
+       GLOBALS()
+       SEP ()
+    POST [ tptr tvoid ] EX p : val, 
+       PROP ()
+       LOCAL (temp ret_temp p)
+       SEP (if eq_dec p nullval then emp
+            else data_at_ Ews (Tstruct _ASN__PRIMITIVE_TYPE_s noattr) p).
+
+Definition Gprog := ltac:(with_library prog [(_calloc, calloc_spec_prim);
                                               ber_check_tags_spec; 
                                               ber_decode_primitive_spec]).
 
@@ -102,7 +148,7 @@ Proof.
   rename H1 into Size.
   rename H2 into Len.
   repeat forward.
-  forward_if (EX p : val, EX ls : list int,
+  forward_if (EX p : val,
   PROP (if eq_dec st_p nullval 
         then p <> nullval 
         else (p = st_p /\ st_p <> nullval))
@@ -116,33 +162,41 @@ Proof.
          temp _opt_codec_ctx ctx_p;
          lvar _rval (Tstruct _asn_dec_rval_s noattr) v_rval;
          temp _td td_p;
-         temp _buf_ptr buf_p; temp _size (Vint (Int.repr size));
+         temp _buf_ptr buf_p;
+         temp _size (Vint (Int.repr size));
          temp _tag_mode (Vint (Int.repr tag_mode)))
   SEP (data_at_ Tsh (Tstruct _asn_dec_rval_s noattr) v__res__1;
        data_at_ Tsh (Tstruct _asn_dec_rval_s noattr) v_tmp_error__2;
        data_at_ Tsh (Tstruct _asn_dec_rval_s noattr) v_tmp_error__1;
        data_at_ Tsh (Tstruct _asn_dec_rval_s noattr) v_tmp_error;
        data_at_ Tsh tint v_length; 
-       data_at_ Tsh (Tstruct _asn_dec_rval_s noattr) v_rval; valid_pointer st_p;
+       data_at_ Tsh (Tstruct _asn_dec_rval_s noattr) v_rval;
+       valid_pointer st_p;
        data_at Tsh asn_codec_ctx_s (Vint (Int.repr ctx)) ctx_p;
-       data_at_ Tsh type_descriptor_s td_p;
-       data_at Tsh (tarray tuchar (Zlength buf)) (map Vint (map Int.repr buf)) buf_p;
+       data_at Tsh (tarray tuint (Zlength (tags td)))
+                  (map Vint (map Int.repr (tags td))) tags_p;
+       field_at Tsh (Tstruct ber_decoder._asn_TYPE_descriptor_s noattr)
+                (DOT ber_decoder._tags) tags_p td_p ;
+       field_at Tsh (Tstruct ber_decoder._asn_TYPE_descriptor_s noattr)
+                   (DOT ber_decoder._tags_count)
+                   (Vint (Int.repr (Zlength (tags td)))) td_p; 
+       data_at Tsh (tarray tuchar (Zlength buf))
+               (map Vint (map Int.repr buf)) buf_p;
        data_at Tsh (tptr tvoid) p st_pp;
        data_at_ Tsh asn_dec_rval_s res_p;
        if eq_dec st_p nullval 
-       then data_at Ews (tarray tint 1) (map Vint ls) p 
-       else data_at_ Ews tint st_p
+       then data_at_ Ews (Tstruct _ASN__PRIMITIVE_TYPE_s noattr) p 
+       else data_at_ Ews (Tstruct _ASN__PRIMITIVE_TYPE_s noattr) st_p
        ))%assert; try congruence.
-  *  (* _st = NULL *)
-    
+  *  (* _st = NULL *)   
     forward_call (1, sizeof (Tstruct _ASN__PRIMITIVE_TYPE_s noattr),
                   (Tstruct _ASN__PRIMITIVE_TYPE_s noattr)).
     cbn; try nia.
     Intros p.
     repeat forward.
-    forward_if ( (PROP ( 
-                      (fst p <> nullval))
-     LOCAL (temp _st (fst p); temp _t'19 st_p;
+    forward_if (
+     (PROP ((p <> nullval))
+     LOCAL (temp _st p; temp _t'19 st_p;
      lvar __res__1 (Tstruct _asn_dec_rval_s noattr) v__res__1;
      lvar _tmp_error__2 (Tstruct _asn_dec_rval_s noattr) v_tmp_error__2;
      lvar _tmp_error__1 (Tstruct _asn_dec_rval_s noattr) v_tmp_error__1;
@@ -150,22 +204,30 @@ Proof.
      lvar _rval (Tstruct _asn_dec_rval_s noattr) v_rval; temp __res res_p;
      temp _opt_codec_ctx ctx_p; temp _td td_p; temp _sptr st_pp; temp _buf_ptr buf_p;
      temp _size (Vint (Int.repr size)); temp _tag_mode (Vint (Int.repr tag_mode)))
-     SEP (if eq_dec (fst p) nullval
+     SEP (if eq_dec p nullval
           then emp
-          else data_at Ews (tarray tint 1) (map Vint (snd p)) (fst p);
+          else data_at_ Ews (Tstruct _ASN__PRIMITIVE_TYPE_s noattr) p;
      data_at_ Tsh (Tstruct _asn_dec_rval_s noattr) v__res__1;
      data_at_ Tsh (Tstruct _asn_dec_rval_s noattr) v_tmp_error__2;
      data_at_ Tsh (Tstruct _asn_dec_rval_s noattr) v_tmp_error__1;
      data_at_ Tsh (Tstruct _asn_dec_rval_s noattr) v_tmp_error;
      data_at Tsh tint (Vint (Int.repr 0)) v_length;
      data_at_ Tsh (Tstruct _asn_dec_rval_s noattr) v_rval; valid_pointer st_p;
-     if eq_dec st_p nullval then emp else data_at_ Ews tint st_p;
+     if eq_dec st_p nullval then emp else data_at_ Ews (Tstruct _ASN__PRIMITIVE_TYPE_s noattr) st_p;
      data_at Tsh asn_codec_ctx_s (Vint (Int.repr ctx)) ctx_p;
-     data_at_ Tsh type_descriptor_s td_p;
-     data_at Tsh (tarray tuchar (Zlength buf)) (map Vint (map Int.repr buf)) buf_p;
+     data_at Tsh (tarray tuint (Zlength (tags td)))
+             (map Vint (map Int.repr (tags td))) tags_p;
+     field_at Tsh (Tstruct ber_decoder._asn_TYPE_descriptor_s noattr)
+              (DOT ber_decoder._tags) tags_p td_p ;
+     field_at Tsh (Tstruct ber_decoder._asn_TYPE_descriptor_s noattr)
+                   (DOT ber_decoder._tags_count)
+                   (Vint (Int.repr (Zlength (tags td)))) td_p; 
+     data_at Tsh (tarray tuchar (Zlength buf)) (map Vint (map Int.repr buf))
+             buf_p;
      data_at Tsh (tptr tvoid) st_p st_pp; data_at_ Tsh asn_dec_rval_s res_p))). 
     break_if. erewrite e. entailer!. entailer!.
     Require Import Forward.
+    (* valid pointer p *) admit.
     match goal with
     | [ _ : _ |- semax _ ?Pre ((Sloop _ Sbreak)) _ ] =>
       forward_loop Pre 
@@ -181,8 +243,8 @@ Proof.
       entailer!.
       forward. entailer!.
       repeat forward.
-      Exists nullval (map Vint (snd p)).
-      repeat rewrite_if_b.
+      Exists nullval.
+ (*     repeat rewrite_if_b.
       entailer!.
     -- (* maloc returned non-null value *)
       forward.
@@ -191,7 +253,7 @@ Proof.
        Exists (fst p) (snd p).
        erewrite H0 in *.
        repeat rewrite_if_b.
-       entailer!. 
+       entailer!.
   * (* st_p <> nullval *)
     rewrite if_false in * by assumption.
     forward.
@@ -202,37 +264,46 @@ Proof.
     forward_empty_loop.
     destruct buf_p; cbn in H3; try contradiction.
     deadvars!.
-    Set Ltac Backtrace.
-    (* FIX forward call - see Boolean decoder in feature/boolean_vst *)
-    forward_call (ctx_p, (Vint (Int.repr ctx)), td_p, td, Vzero, Vzero, b, i, buf,
-                  v__res__1, size, tag_mode, 0, v_length, Vzero, 0%Z).
+    forward_call (ctx_p,
+                  td_p, td, tags_p, Vzero, b, i, buf,
+                  v__res__1, size, tag_mode, 0, v_length, Vzero, ctx%Z).
+    Require Import Core.Tactics.
+    repeat split; auto; try lia; strip_repr_ptr.
+    cbn in H7.
+    strip_repr.
     break_if.
-    ** 
-    inversion H0. 
-    pose proof Exec.ber_check_tags_bool_res td buf DT as BCT.
-    inversion BCT as [T | T]; rewrite T in *;
-        unfold mk_dec_rval, tag_length, tag_consumed.
+    ** break_match.  
       2: { (* If ber_check_tags failed *)
-        normalize;
+        normalize.
+        unfold mk_dec_rval.
+        unfold asn_dec_rval_s.
         repeat forward.
         all: forward_if; [|discriminate];
           repeat forward.
         Exists p (map Vint ls).
         rewrite if_false by assumption.
-        unfold bool_decoder; rewrite T; 
-          destruct buf; entailer!. 
-        simpl.
-        entailer!. }
+        unfold primitive_decoder.
+        replace (map Int.repr (map Byte.unsigned (map Byte.repr buf)))
+                with (map Int.repr buf).
+        rewrite Heqo.
+          destruct buf;  erewrite <- H32; entailer!.  
+        simpl. entailer!.
+        f_equal.
+        (* check types byte v. int in ber_check_tags *)
+        admit.
+ }
       (* If ber_check_tags succeded *)
       { 
-        clear BCT; rename T into BCT; cbn in Size; subst.
+        rename Heqo into BCT; cbn in Size; subst.
         normalize.
+        change_compspecs CompSpecs.
         repeat forward.
         forward_if; [congruence|].
         forward_empty_loop.
         repeat forward.
         forward_if.
         (* RW_MORE case *) admit.
+        forward.
         forward.
         forward_if True. 
       (* if length <> 1 *)
@@ -377,6 +448,6 @@ Proof.
       rewrite Z.
       simpl.
       rewrite if_false in * by assumption.
-      entailer!. *)
+      entailer!.  *)
 Admitted.
  End Ber_decode_primitive.
